SkLean/tests/Dsl.lean
@@ -1,7 +1,0 @@
-import SkLean.Dsl
-
-#eval SK[K]
-#eval SK[S]
-#eval SK[∀ x : Prop, (∀ y : #x, Prop)]
-#eval SK[∀ α : #α, (∀ β : #β, (∀ x : #α, (∀ y : #β, #α)))]
-#eval SK[Prop → Prop]
